\section*{Aufgabe 3.1}
\subsection*{1)}
$(h \circ val)^* = h \circ val^*\\
\\
(h \circ val)^* : T_{\Sigma}(V) \rightarrow B\\
h \circ val : V \rightarrow B\\
h : A \rightarrow B\\
val : V \rightarrow A\\
val^* : T_\Sigma(V) \rightarrow A\\
\\
\text{Annahme: } h^* \text{ ist definiert als:}\\
\forall h : A \rightarrow B \text{ sei ein } \Sigma$-Homomorphismus, $A$ und $B$ seien $S$-Sortige Mengen.$\\
h^* : T_\Sigma(A) \rightarrow B\\
\forall a\in A: h^*(a) = h(a)\\
\forall f: e \rightarrow e' \in F, $ und $ t \in T_\Sigma(A)_e: h_{e'}^*(f(t)) = f^A(h_e^*(t))\\
\\
$Falls $ x\in V:\\
(h\circ val)^*(x) = (h\circ val)(x) = h(val(x)) = h(val^*(x)) = h\circ val^* \\
$Sei $f:e\rightarrow e' \in F$ und $t\in T_\Sigma(V)_e\\
(h\circ val^*)(f(t))=h(val^*(f(t)))=h(f^A(val^*(t)))=f^B(h(val^*(t)))=f^B((h\circ val^*)(t)) = f^B((h\circ val)^*(t)) =(h\circ val)^*(f(t))$
\subsection*{2)}
$h\circ t^A = t^B \circ h\\
t^A:A^n\rightarrow A\\
(a_1,\dots a_n) \mapsto val^*(t)\\
h:A\rightarrow B\\
(h\circ t^A) = (h\circ val^{A*})(f(t)) = h(val^{A*}(f(t))) = val^{B*}(h(f(t))) = (val^{B*} \circ h)(f(t))=(t^B\circ h)$
