\newpage
\section*{Aufgabe 2.2}
\begin{tabular}{rl}
Expr $\rightarrow$ & Term Expr'\\
Expr' $\rightarrow$& + Term Expr' | - Term Expr' | $\epsilon$\\
Term $\rightarrow$& Factor Term'\\
Term' $\rightarrow$& * Factor Term' | / Factor Term' | $\epsilon$\\
Factor $\rightarrow$& ( Expr ) | Int
\end{tabular}

\subsection*{1)}
Die Abstrakte Syntax von G:\\
$\Sigma(G) = (\{Expr, Expr', Term, Term', Factor\},\{Int\},\{\\
\_ \_ : Term Expr' \rightarrow Expr,\\
+ \_ \_ : Term Expr' \rightarrow Expr',\\
- \_ \_ : Term Expr' \rightarrow Expr',\\
1 : 1 \rightarrow Expr',\\
\_ \_ : Factor Term' \rightarrow Term,\\
* \_ \_ : Factor Term' \rightarrow Term',\\
/ \_ \_ : Factor Term' \rightarrow Term',\\
1 : 1 \rightarrow Term',\\
( \_ ) : Expr \rightarrow Factor,\\
int : Int \rightarrow Factor\}$\\

$\Sigma$-Grundtermalgebra $T_\Sigma=(A,OP)$ mit
\[A=\{A_{Expr}, A_{Expr'}, A_{Term}, A_{Term'}, A_{Factor}\}\]
\[OP=\{\_ \_^{T_\Sigma} = \_ \_,
+ \_ \_^{T_\Sigma} = + \_ \_,
- \_ \_^{T_\Sigma} = + \_ \_,
1^{T_\Sigma} = 1,
\_ \_^{T_\Sigma} = \_ \_
...\}\]
\subsection*{2)} %Das ist irgendwie so im Skript notiert, aber das mach einfach keinen Sinn....
$Word(G)_{Expr}=(Z\cup \bigcup BS)^*=\{Int,+,-,*,/,(,)\}^*\\
Word(G)_{Expr'}=\{Int,+,-,*,/,(,)\}^*\\
Word(G)_{Term}=\{Int,+,-,*,/,(,)\}^*\\
Word(G)_{Term'}=\{Int,+,-,*,/,(,)\}^*\\
Word(G)_{Factor}=\{Int,+,-,*,/,(,)\}^*\\$
%(2+3)*4

%    _ _
%   /   \
%  _ _   1


%   * _ _
%   /   \
%( _ )  Int
%  |
%+ _ _
% /  \
%Int Int


