\section*{Aufgabe 5.2}
\[d(0,m)=0\]
\[d(s(n),0)=s(n)\]
\[d(s(n),s(m))=d(n,m)\]

\[\text{adiff}(n,m)=\begin{cases}
0&$ falls $ n<m\\
n-m& $ansonsten$
\end{cases}\]
\\
Induktionsanfang: \\
$d(0,m)=0=$ adiff$(0,m)$ da $0<=m$\\
$d(s(n),0)=s(n)=s(n)-0=$ adiff$(s(n),0)$\\
Induktionsschritt:\\
Für $n<=m$\\
$d(n,m)=$ adiff$(n,m)=n-m$\\
$\Rightarrow d(s(n),s(m))=$ adiff$(n,m)=n-m=s(n)-s(m)=$ adiff$(s(n),s(m))$\\
Für $n>m$:\\
$d(n,m)=$ adiff$(n,m)=0$\\
$\Rightarrow d(s(n),s(m))=$ adiff$(n,m)=0=$ adiff$(s(n),s(m))$\\
