\section*{Aufgabe 9.1}
\[G=(\{Expr, Expr', Term, Term', Factor\},\{\mathbb{Z}\},\{+,-,*,/,(,)\},R\})\]
R:\\
Expr -> Term Expr'\\
Expr' -> + Term Expr' | $\epsilon$\\
Term -> Factor Term'\\
Term' -> * Factor Term' | $\epsilon$\\
Factor -> ( Expr ) | $\mathbb{Z}$\\
\subsection*{9.1.1}
$\Sigma(G)=(\{Expr, Expr', Term, Term', Factor\},\{\mathbb{Z}\},F)$\\
$F=\{\\
mkExpr : Term \times Expr' \rightarrow Expr\\
plusExpr' : Term \times Expr' \rightarrow Expr'\\
mtExpr' : 1 \rightarrow Expr'\\
mkTerm : Factor \times Term' \rightarrow Term\\
multTerm' : Factor \times Term' \rightarrow Term'\\
mtTerm' : 1 \rightarrow Term'\\
exp2fac : Expr \rightarrow Factor\\
z2fac : \mathbb{Z} \rightarrow Factor\\ \}$
\subsection*{9.1.2}
$R=\{\\
r_{11}=(Expr\rightarrow Term\: Expr'),\\
r_{21}=(Expr'\rightarrow +\: Term\: Expr'), r_{22}=(Expr'\rightarrow\epsilon),\\
r_{31}=(Term\rightarrow Factor\: Term'),\\
r_{41}=(Term'\rightarrow *\: Factor\: Term'), r_{42}=(Term'\rightarrow\epsilon),\\
r_{51}=(Factor\rightarrow (\: Expr\: )\:), r_{52}=(Factor\rightarrow\mathbb{Z}),\\
\}\\
\\
\text{Für }x\in X, w\in X^*\\
\\
compStep_{Expr}(w)=msum[try_{r_{11}}(w)]\\
compStep_{Expr'}(w)=msum[try_{r_{21}}(w), try_{r_{22}}(w)]\\
compStep_{Term}(w)=msum[try_{r_{31}}(w)]\\
compStep_{Term'}(w)=msum[try_{r_{41}}(w), try_{r_{42}}(w)]\\
compStep_{Factor}(w)=msum[try_{r_{51}}(w), try_{r_{52}}(w)]\\
compStep_{\mathbb{Z}}(xw)=\:if x\in\mathbb{Z} \:then \:return (x,w) \:else \:fail(x\notin\mathbb{Z})\\
compStep_{\mathbb{Z}}(\epsilon)=fail(no input)\\
compStep_{+}(xw)=\:if\: x = + \:then\: return(x,w) \:else \:fail(x\neq +)\\
compStep_{+}(\epsilon)=fail(no input)\\
compStep_{-}(xw)=\:if\: x = - \:then\: return(x,w) \:else \:fail(x\neq -)\\
compStep_{-}(\epsilon)=fail(no input)\\
compStep_{*}(xw)=\:if\: x = * \:then\: return(x,w) \:else \:fail(x\neq *)\\
compStep_{*}(\epsilon)=fail(no input)\\
compStep_{/}(xw)=\:if\: x = / \:then\: return(x,w) \:else \:fail(x\neq /)\\
compStep_{/}(\epsilon)=fail(no input)\\
compStep_{(}(xw)=\:if\: x = ( \:then\: return(x,w) \:else \:fail(x\neq ()\\
compStep_{(}(\epsilon)=fail(no input)\\
compStep_{)}(xw)=\:if\: x = ) \:then\: return(x,w) \:else \:fail(x\neq ))\\
compStep_{)}(\epsilon)=fail(no input)\\
\\
try_{r_{11}}(w)=compStep_{Term}(w) >>= \lambda(a_1,w).(compStep_{Expr'}(w) >>= \lambda(a_2,w).(mkExpr(a_1,a_2)))\\
try_{r_{21}}(w)=compStep_{+}(w) >>= \lambda(a_1,w).(compStep_{Term}(w) >>= \lambda(a_2,w).(compStep_{Expr'}(w) >>= \lambda(a_3,w).(plusExpr'(a_2,a_3))))\\
try_{r_{22}}(w)=return(mtExpr', w)\\
try_{r_{31}}(w)=compStep_{Factor}(w) >> \lambda(a_1,w).(compStep_{Term'}(w) >>= \lambda(a_2,w).(mkTerm(a_1,a_2)))\\
try_{r_{41}}(w)=compStep_{*}{w} >>= \lambda(a_1,w).(compStep_{Factor}(w) >>= \lambda(a_2,w).(compStep_{Term'}(w) >>= \lambda(a_3,w).(multTerm'(a_2,a_3))))\\
try_{r_{42}}(w)=return(mtTerm', w)\\
try_{r_{51}}(w)=compStep_((w) >>= \lambda(a_1,w).(compStep_{Expr}(w) >>= \lambda(a_2,w).(compStep_)(w) >>= \lambda(a_3,w).(exp2fac(a_2))))\\
try_{r_{52}}(w)=compStep_{\mathbb{Z}}(w) >>= \lambda(a_1,w).z2fac(a_1)\\
\\
compile^{Ziel}_{G,Expr}=compStep_{Expr}(w) >>= \lambda(a,w).\:if\:w=\epsilon\:then\:return(a)\:else\:fail(w)\\
compile^{Ziel}_{G,Expr'}=compStep_{Expr'}(w) >>= \lambda(a,w).\:if\:w=\epsilon\:then\:return(a)\:else\:fail(w)\\
compile^{Ziel}_{G,Term}=compStep_{Term}(w) >>= \lambda(a,w).\:if\:w=\epsilon\:then\:return(a)\:else\:fail(w)\\
compile^{Ziel}_{G,Term'}=compStep_{Term'}(w) >>= \lambda(a,w).\:if\:w=\epsilon\:then\:return(a)\:else\:fail(w)\\
compile^{Ziel}_{G,Factor}=compStep_{Factor}(w) >>= \lambda(a,w).\:if\:w=\epsilon\:then\:return(a)\:else\:fail(w)\\
compile^{Ziel}_{G,\mathbb{Z}}=compStep_{\mathbb{Z}}(w) >>= \lambda(a,w).\:if\:w=\epsilon\:then\:return(a)\:else\:fail(w)\\
compile^{Ziel}_{G,+}=compStep_{+}(w) >>= \lambda(a,w).\:if\:w=\epsilon\:then\:return(a)\:else\:fail(w)\\
compile^{Ziel}_{G,-}=compStep_{-}(w) >>= \lambda(a,w).\:if\:w=\epsilon\:then\:return(a)\:else\:fail(w)\\
compile^{Ziel}_{G,*}=compStep_{*}(w) >>= \lambda(a,w).\:if\:w=\epsilon\:then\:return(a)\:else\:fail(w)\\
compile^{Ziel}_{G,/}=compStep_{/}(w) >>= \lambda(a,w).\:if\:w=\epsilon\:then\:return(a)\:else\:fail(w)\\
compile^{Ziel}_{G,(}=compStep_{(}(w) >>= \lambda(a,w).\:if\:w=\epsilon\:then\:return(a)\:else\:fail(w)\\
compile^{Ziel}_{G,)}=compStep_{)}(w) >>= \lambda(a,w).\:if\:w=\epsilon\:then\:return(a)\:else\:fail(w)\\
$
\subsection*{9.1.3}
$compile^{T_{\Sigma(G)}}_G=parse_G$\\
$parse_G(8+3*4)$ gibt den folgenden Syntaxbaum:\\
\begin{tikzpicture}[level/.style={sibling distance=60mm/#1}]
\node (z){mkExpr}
  child {node (a) {mkTerm}
    child {node (b) {z2fac}
      child {node {8}}}
    child {node {mtTerm'}}}
  child {node {plusExpr'}
    child {node {mkTerm}
      child {node {z2fac}
        child {node {3}}}
      child {node {multTerm'}
        child {node {z2fac}
          child {node {4}}}
        child {node {mtTerm'}}}}
  child {node {mtExpr'}}
};
\end{tikzpicture}
\section*{Aufgabe 9.2}
Füge die Regel $start\rightarrow Expr$ zu $R$ hinzu\\
$first(start)=\{(,\mathbb{Z}\}\\
first(Expr)=\{(,\mathbb{Z}\}\\
first(Expr')=\{\epsilon,+\}\\
first(Term)=\{(,\mathbb{Z}\}\\
first(Term')=\{\epsilon,*\}\\
first(Factor)=\{(,\mathbb{Z}\}\\
\text{Für }w\in BS^*\\
first(+w)=\{+\}\\
first(-w)=\{-\}\\
first(*w)=\{*\}\\
first(/w)=\{/\}\\
first((w)=\{(\}\\
first()w)=\{)\}\\
\\
follow(start)=\emptyset\\
follow(Expr)=\{)\}\\
follow(Expr')=\{)\}\\
follow(Term)=\{+,)\}\\
follow(Term')=\{+,)\}\\
follow(Factor)=\{*,+,)\}\\$
